client.v
@@ -1,17 +1,219 @@
+Require Import List.
+Import ListNotations.
+
 Require Import ZArith.
 Require Import String.
+Require Import Bool.
 
 AddPath "/Users/joald/wwk/client" as.
 
 Load packet.
 
+Open Scope list_scope.
+
+Inductive directive : Set :=
+| SEND_PACKET
+| WRITE_CONTENTS
+| SEND_TO : positive -> directive
+| PRINT.
+
 Record state : Set := mkState {
+  orders : list directive;
   transfer_mode : mode;
   port: option positive;
-  last_packet : option packet;
-  timeout_count : N;
+  last_packet : packet;
+  last_block_id : N;
+  did_retransmit : bool;
+  finished : bool;
   file_contents : string;
 }.
+
+
+Record result := mkResult {
+  (* the packet that the client needs to send next *)
+  packet_to_send : string; 
+
+  (* next state *)
+  new_state : state;
+}.
+
+(** When reading:
+  - in_file is the name of the file on the server.
+  - out_file is the name of the file on the local machine.
+    When writing:
+  - in_file is the contents of the file on the local machine.
+  - out_file is the name of the file on the server
+*)
+Definition coq_init (rw_mode : mode) (in_file : string) (out_file : string) : result := 
+  let pac := init_packet rw_mode in_file out_file in
+  mkResult
+    (serialize_packet pac)
+    (mkState ([SEND_PACKET]) rw_mode None pac 0 false false
+      match rw_mode with
+      | Read => ""
+      | Write => in_file
+      end).
+
+Theorem init_when_reading_infile_is_in_packet : forall infil outfil, 
+  let p := packet_to_send (coq_init Read infil outfil) in
+  substring 2 (length infil) p = infil.
+Proof.
+intros.
+magic.
+elim infil.
+* magics.
+* magic.
+  rewrite H.
+  auto.
+Qed.
+
+Theorem init_when_reading_file_contents_is_empty : forall infil outfil,
+  file_contents (new_state (coq_init Read infil outfil)) = EmptyString.
+Proof. magic. Qed.
+
+Theorem init_when_writing_out_file_is_in_packet : forall infil outfil, 
+  let p := packet_to_send (coq_init Write infil outfil) in
+  substring 2 (length outfil) p = outfil.
+Proof.
+intros.
+magic.
+elim outfil.
+* magics.
+* magic.
+  rewrite H.
+  auto.
+Qed.
+
+Theorem init_when_writing_file_contents_is_infile : forall infil outfil,
+  file_contents (new_state (coq_init Write infil outfil)) = infil.
+Proof. magic. Qed.
+
+Definition illegal_operation (err_msg : string) (st : state) : result := mkResult
+  (serialize_packet (p_ERROR ILLEGAL_TFTP_OPERATION err_msg))
+  (mkState [SEND_PACKET] (transfer_mode st) (port st) (last_packet st) (last_block_id st) false true "").
+
+Definition wrong_source_port (st : state) (p : positive) : result := mkResult 
+  (serialize_packet (p_ERROR UNKNOWN_TRANSFER_ID ""))
+  (mkState [SEND_TO p] (transfer_mode st) (port st) (last_packet st) (last_block_id st) (did_retransmit st) (finished st) (file_contents st)).
+
+Definition request_retransmit (st : state) : result := 
+  if did_retransmit st
+    then mkResult "The server timed out."
+      (mkState [PRINT] (transfer_mode st) (port st) (last_packet st) (last_block_id st) true true "")
+    else mkResult 
+      (serialize_packet (last_packet st))
+      (mkState [SEND_PACKET] (transfer_mode st) (port st) (last_packet st) (last_block_id st) true (finished st) (file_contents st)).
+
+Definition send_bytes (st : state) (byte_count : nat) : forall new_id, new_id < two_bytes_range_size -> result := fun new_id prop =>
+  let to_send := substring 0 byte_count (file_contents st) in
+  let rest    := substring byte_count (length (file_contents st) - byte_count) (file_contents st) in
+  let pac     := p_DATA new_id prop to_send in
+  mkResult
+    (serialize_packet pac)
+    (mkState [SEND_PACKET] Write (port st) pac new_id false (N_of_nat byte_count <? 512) rest).
+
+Definition coq_process_packet (pack : string) (st : state) (p : positive) (timeout : bool) : result.
+Proof.
+Open Scope positive_scope.
+refine (
+  if finished st
+    then mkResult "" st
+    else _
+).
+refine (
+  if timeout 
+    then request_retransmit st 
+    else _
+).
+refine (
+  if (
+    match port st with 
+    | None => false 
+    | Some p2 => negb (Pos.eqb p p2)
+    end 
+  ) then wrong_source_port st p
+    else _
+).
+destruct (deserialize_packet pack).
++ destruct p0.
+  - exact (illegal_operation "Cannot send read requests to client." st).
+  - exact (illegal_operation "Cannot send write requests to client." st).
+  - (* p_DATA *)
+    remember x as nr.
+    remember l as prop.
+    remember s as data.
+
+    refine (
+      match transfer_mode st with
+      | Read => _
+      | Write => illegal_operation "Cannot receive data in write mode." st
+      end
+    ).
+    Local Close Scope positive_scope.
+    Local Open Scope N_scope.
+    refine (
+      if nr =? last_block_id st + 1
+        then _
+        else illegal_operation "Incorrect block number." st
+    ).
+    refine (
+      if negb (N_of_nat (length data) =? 512)
+        then mkResult "" (mkState [WRITE_CONTENTS] Read (port st) 
+          (last_packet st) nr false true (file_contents st ++ data))
+        else let pac := (p_ACK nr prop) in
+          mkResult (serialize_packet pac)
+            (mkState [SEND_PACKET] Read (Some p) pac nr 
+                false false (file_contents st ++ data))
+    ).
+  - (* p_ACK *)
+    remember x as nr.
+    refine (
+      match transfer_mode st with
+      | Read => illegal_operation "Cannot receive data in write mode." st
+      | Write => _
+      end
+    ).
+    case_eq (two_bytes_range_size ?= nr + 1).
+    * intro.
+      assert (two_bytes_range_size = nr + 1).
+      { apply (N.compare_eq_iff two_bytes_range_size (nr + 1)).
+        assumption. }
+      exact (illegal_operation "File too large." st).
+    * intro.
+      assert (two_bytes_range_size < nr + 1).
+      { apply (N.compare_lt_iff two_bytes_range_size (nr + 1)).
+        assumption. }
+      exact (illegal_operation "File too large." st).
+    * intro.
+      assert (nr + 1 < two_bytes_range_size).
+      { apply (N.compare_gt_iff two_bytes_range_size (nr + 1)).
+        assumption. }
+      remember (N_of_nat (length (file_contents st))) as CL.
+      case_eq (CL ?= 512).
+      -- intro.
+         assert (CL = 512).
+         { apply (N.compare_eq_iff CL 512).
+           assumption. }
+         exact (send_bytes st 512 (nr + 1) H0).
+      -- intro.
+         assert (CL < 512).
+         { apply (N.compare_lt_iff CL 512).
+           assumption. } 
+         exact (send_bytes st (nat_of_N CL) (nr + 1) H0).
+      -- intro.
+         assert (512 < CL).
+         { apply (N.compare_gt_iff CL 512).
+           assumption. } 
+         exact (send_bytes st 512 (nr + 1) H0).
+  - (* p_ERROR *)
+    remember s as err_msg.
+    exact (
+      mkResult err_msg
+        (mkState [PRINT] (transfer_mode st) (port st) (last_packet st) (last_block_id st) false true (file_contents st))
+    ).
+
++ exact (illegal_operation "Cannot understand package." st).
+Defined.
 
 (*
 Inductive packet : Set := 
@@ -20,23 +222,21 @@ Inductive packet : Set :=
 | p_DATA : forall (x : N), x < two_bytes_range_size -> string -> packet     (* Block #, Data *)
 | p_ACK : forall (x : N), x < two_bytes_range_size -> packet                (* Block # *)
 | p_ERROR : error_code -> string -> packet. (* ErrorCode, ErrMsg *)
-*)
 
-Record result := mkResult {
-  packet_to_send : option packet;
-  new_state : option state;
-  file_data : option string;
+Record state : Set := mkState {
+  orders : list directive;
+  transfer_mode : mode;
+  port: option positive;
+  last_packet : packet;
+  did_retransmit : bool;
+  finished : bool;
+  file_contents : string;
 }.
+Record result := mkResult {
+  (* the packet that the client needs to send next *)
+  packet_to_send : string; 
 
-(** When reading:
-  - in_file is the name of the file on the server.
-  - out_file is the name of the file on the local machine.
-  When writing:
-  - in_file is the contents of the file on the local machine.
-  - out_file is the name of the file on the server
+  (* next state *)
+  new_state : state;
+}.
 *)
-Definition coq_init (rw_mode : mode) (in_file : string) (out_file : string) : result := 
-  (serialize_packet (init_packet mode in_file out_file), 
-   mkState mode None None (?) match
-
-Definition coq_process_state () := .
